src/priority.v
@@ -1,0 +1,182 @@
+From Coq Require Import ssreflect ssrbool ssrfun.
+From mathcomp Require Import eqtype order seq path.
+From favssr Require Import prelude bintree.
+
+Set Implicit Arguments.
+Unset Strict Implicit.
+Unset Printing Implicit Defensive.
+
+Import Order.POrderTheory.
+Import Order.TotalTheory.
+Open Scope order_scope.
+
+Module APQ.
+Structure APQ (disp : unit) (T : orderType disp): Type :=
+  make {tp :> Type;
+        empty : tp;
+        insert : T -> tp -> tp;
+        del_min : tp -> tp;
+        get_min : T -> tp -> T;
+
+        mset : tp -> seq T;
+        invar : tp -> bool;
+
+        _ : invar empty;
+        _ : mset empty = [::];
+
+        _ : forall x s, invar s -> invar (insert x s);
+        _ : forall x s, invar s ->
+              perm_eq (mset (insert x s)) (x :: mset s);
+
+        _ : forall s, invar s -> ~~ nilp (mset s) -> invar (del_min s);
+        _ : forall x0 s, invar s -> ~~ nilp (mset s) ->
+              perm_eq (mset (del_min s)) (rem (get_min x0 s) (mset s));
+
+        (* we don't need non-emptiness here since we've made both sides total *)
+        _ : forall s x0, invar s ->
+              get_min x0 s = mins x0 (mset s)
+        }.
+End APQ.
+
+Module APQM.
+Structure APQ (disp : unit) (T : orderType disp): Type :=
+  make {tp :> Type;
+        empty : tp;
+        insert : T -> tp -> tp;
+        del_min : tp -> tp;
+        get_min : T -> tp -> T;
+        meld : tp -> tp -> tp;
+
+        mset : tp -> seq T;
+        invar : tp -> bool;
+
+        _ : invar empty;
+        _ : mset empty = [::];
+
+        _ : forall x s, invar s -> invar (insert x s);
+        _ : forall x s, invar s ->
+              perm_eq (mset (insert x s)) (x :: mset s);
+
+        _ : forall s, invar s -> ~~ nilp (mset s) -> invar (del_min s);
+        _ : forall x0 s, invar s -> ~~ nilp (mset s) ->
+              perm_eq (mset (del_min s)) (rem (get_min x0 s) (mset s));
+
+        _ : forall s x0, invar s ->
+              get_min x0 s = mins x0 (mset s);
+
+        _ : forall s1 s2, invar s1 -> invar s2 -> invar (meld s1 s2);
+        _ : forall s1 s2, invar s1 -> invar s2 ->
+              perm_eq (mset (meld s1 s2)) (mset s1 ++ mset s2)
+
+        }.
+End APQM.
+
+(* Exercise 14.1 *)
+Section Exercise.
+Context {disp : unit} {T : orderType disp}.
+
+Definition empty_list : seq T := [::].
+
+Fixpoint ins_list (x : T) (xs : seq T) : seq T := xs. (* FIXME *)
+
+Definition del_min_list (xs : seq T) : seq T := xs. (* FIXME *)
+
+Definition get_min_list (x0 : T) (xs : seq T) : T := x0. (* FIXME *)
+
+Definition invar_list (t : seq T) : bool := true. (* FIXME *)
+
+Definition merge_list (xs1 xs2 : seq T) : seq T := xs1. (* FIXME *)
+
+(* PROVE PROPERTIES *)
+
+Definition ListPQM :=
+  @APQM.make _ _ (seq T)
+  empty_list ins_list del_min_list get_min_list merge_list
+  id invar_list
+  (* use proved lemmas *)
+  .
+
+End Exercise.
+
+Section Heaps.
+Context {disp : unit} {T : orderType disp}.
+
+Fixpoint heap (t : tree T) : bool :=
+  if t is Node l m r
+    then [&& all (>= m) (inorder l ++ inorder r), heap l & heap r]
+    else true.
+
+Definition mset_tree : tree T -> seq T := preorder.
+
+Definition empty : tree T := leaf.
+
+Definition get_min (x0 : T) (t : tree T) : T :=
+  if t is Node _ x _
+    then x else x0.
+
+Fixpoint meld (t1 : tree T) :=
+  if t1 is Node l1 a1 r1 then
+    let fix meld_t1 t2 :=
+      if t2 is Node l2 a2 r2 then
+        if a1 <= a2 then Node l1 a1 (meld r1 t2) else Node l2 a2 (meld_t1 r2)
+      else t1 in
+    meld_t1
+  else id.
+
+Definition insert x t := meld (Node leaf x leaf) t.
+
+Definition del_min (t : tree T) : tree T :=
+  if t is Node l _ r then meld l r else leaf.
+
+(* Exercise 14.2 *)
+
+Lemma invar_empty : heap empty.
+Proof. Admitted.
+
+Lemma mset_empty : mset_tree empty = [::].
+Proof. Admitted.
+
+Lemma invar_meld t1 t2 : heap t1 -> heap t2 -> heap (meld t1 t2).
+Proof.
+Admitted.
+
+Lemma mset_meld t1 t2 : heap t1 -> heap t2 ->
+  perm_eq (mset_tree (meld t1 t2)) (mset_tree t1 ++ mset_tree t2).
+Proof.
+Admitted.
+
+Corollary invar_insert_heap x t : heap t -> heap (insert x t).
+Proof. by rewrite /insert=>H; apply: invar_meld. Qed.
+
+Corollary mset_insert x t : heap t ->
+  perm_eq (mset_tree (insert x t)) (x :: mset_tree t).
+Proof. by rewrite /insert=>H; apply: perm_trans; first by apply: mset_meld. Qed.
+
+Corollary invar_delmin_heap t : heap t -> ~~ nilp (mset_tree t) -> heap (del_min t).
+Proof.
+case: t=>//=l a r; case/and3P=>_ Hl Hr _.
+by apply: invar_meld.
+Qed.
+
+Corollary mset_delmin_heap x0 t : heap t -> ~~ nilp (mset_tree t) ->
+  perm_eq (mset_tree (del_min t)) (rem (get_min x0 t) (mset_tree t)).
+Proof.
+case: t=>//=l a r; case/and3P=>_ Hl Hr _; rewrite eq_refl.
+by apply: mset_meld.
+Qed.
+
+Lemma mins_getmin_heap t x0 : heap t ->
+  get_min x0 t = mins x0 (mset_tree t).
+Admitted.
+
+Definition HeapPQM :=
+  @APQM.make _ _ (tree T)
+    empty insert del_min get_min meld
+    mset_tree heap
+    invar_empty mset_empty
+    invar_insert_heap mset_insert
+    invar_delmin_heap mset_delmin_heap
+    mins_getmin_heap
+    invar_meld mset_meld.
+
+End Heaps.
