README.md
@@ -22,7 +22,7 @@ Besides Mathcomp, this also requires the [Equations](https://mattam82.github.io/
 12. [Tries](src/trie.v)
 13. [Huffman’s Algorithm](src/huffman.v)
 ### Part III: Priority Queues
-14. Priority Queues
+14. [Priority Queues](src/priority.v)
 15. Leftist Heaps
 16. Priority Queues via Braun Trees
 17. Binomial Heaps
